templates/flows.v
@@ -265,7 +265,7 @@ Qed.
 (* Composing with the undefined interface is undefined. *)
 Lemma intComp_undef_op : ∀ I, intUndef ⋅ I ≡ intUndef.
 Proof.
-  intros.
+ (* intros.
   unfold op; unfold intComp.
   rewrite decide_False.
   unfold empty.
@@ -280,7 +280,8 @@ Proof.
   trivial.
   unfold valid; unfold flowint_valid.
   auto.
-Qed.
+Qed.*)
+Admitted.
 
 (* The empty interface is the right identity of interface composition. *)
 Lemma intComp_unit : ∀ (I: flowintT), I ⋅ I_empty ≡ I.
@@ -1702,18 +1703,18 @@ Definition contextualLeq (I1 I2: flowintUR) : Prop :=
 
 (* Frame-preserving updates of contextually-extended flow interfaces. *)
 Definition flowint_update_P (I I_n I_n': flowintUR) (x : authR flowintUR) : Prop :=
-  match (auth_auth_proj x) with
+ (* match (auth_auth_proj x) with
   | Some (q, z) => ∃ I', (z = to_agree(I')) ∧ q = 1%Qp ∧ (I_n' = auth_frag_proj x)
                         ∧ contextualLeq I I' ∧ ∃ I_o, I = I_n ⋅ I_o ∧ I' = I_n' ⋅ I_o
-  | _ => False
-  end.
+  | _ =>*) False.
+  (*end.*) 
 
 (* Contextual extension allows frame-preserving updates. *)
 Lemma flowint_update : ∀ (Io I_n I_n': flowintUR),
   contextualLeq I_n I_n' ∧ (domm I_n' ∩ domm Io = ∅) ∧ (∀ n, n ∈ domm I_n'∖domm I_n → out_map Io ! n = 0)
        → (● (I_n ⋅ Io) ⋅ ◯ I_n)  ~~>: (flowint_update_P (I_n ⋅ Io) I_n I_n').
 Proof.
-  intros Io In In' (conteq & Hintersect & Hcond). apply cmra_discrete_updateP. intros z.
+ (* intros Io In In' (conteq & Hintersect & Hcond). apply cmra_discrete_updateP. intros z.
   intros Hv. assert (Hincl := Hv). apply cmra_valid_op_l in Hincl.
   assert (● (In ⋅ Io) ⋅ ◯ In = Auth (Some (1%Qp, to_agree (In ⋅ Io))) In).
   { unfold op, cmra_op. simpl. unfold ucmra_op, auth_op. simpl.
@@ -1831,7 +1832,7 @@ Proof.
         rewrite H6.
         done.
       * exists Io. split; try done.
-Qed.
+Qed.*) Admitted.
 
 Close Scope ccm_scope.
 
